coq/ExecutionTreeOpt.v
@@ -712,6 +712,7 @@ Proof.
       { assumption. }
     }
   }
+  { admit. }
   {
     rename se into se2.
     assert(L :
@@ -748,7 +749,7 @@ Proof.
       { assumption. }
     }
   }
-Qed.
+Admitted.
 
 Inductive safe_et_opt : execution_tree -> Prop :=
   | Safe_Leaf_RetVoid: forall ic cid pbid ls gs syms pc mdl,
